# 《多体系统的量子场论》4.3.2草稿

(4.3.6)式$(i\partial_ic^\dagger(\pmb x))c(\pmb x)$前应该是正号。

## 问题4.3.3.
1.
$$H=\int d^d\pmb x\ c^\dagger(\pmb x)\epsilon(-i\partial_i+A_i(\pmb x))c(\pmb x)$$

$$H'=\int d^d\pmb x\ \exp[i\phi(\pmb x)]c^\dagger(\pmb x)\times\\\epsilon(-i\partial_i+A_i(\pmb x)+\partial_i\phi(\pmb x))(\exp[-i\phi(\pmb x)]c(\pmb x))$$

$$(-i\partial_i+A_i(\pmb x)+\partial_i\phi(\pmb x))(\exp[-i\phi(\pmb x)]f(\pmb x))\\=-i\exp[-i\phi(\pmb x)]\partial_if(\pmb x)-\exp[-i\phi(\pmb x)]\partial_i\phi(\pmb x)f(\pmb x)\\+\exp[-i\phi(\pmb x)]A_i(\pmb x)f(\pmb x)+\exp[-i\phi(\pmb x)]\partial_i\phi(\pmb x)f(\pmb x)\\=\exp[-i\phi(\pmb x)](-i\partial_i+A_i(\pmb x))f(\pmb x)$$

故
$$\epsilon(-i\partial_i+A_i(\pmb x)+\partial_i\phi(\pmb x))(\exp[-i\phi(\pmb x)]f(\pmb x))\\=\exp[-i\phi(\pmb x)]\epsilon(-i\partial_i+A_i(\pmb x))f(\pmb x)$$

故
$$H'=H$$

2.
由上文可知，如果
$$A_i\to A_i+\partial_i\phi,c\to\exp[-i\phi]c$$

那么
$$H\to H$$

根据定义
$$J^i(\pmb x)=\frac{\delta H}{\delta A_i(\pmb x)}$$

故$A_i$的变化引起的$H$的变化为
$$\int d^d\pmb x\ \pmb J(\pmb x)\cdot\pmb\nabla\phi(\pmb x)+O(\phi^2)\\=-\int d^d\pmb x\ \pmb\nabla\cdot\pmb J(\pmb x)\phi(\pmb x)+O(\phi^2)$$

设
$$G=\int d^d\pmb x\ \phi(\pmb x)\rho(\pmb x)$$

于是
$$\exp[iG]c(\pmb x)\exp[-iG]=\exp[-i\phi(\pmb x)]c(\pmb x)$$

故$c$的变化引起的$H$的变化为
$$\exp[iG]H\exp[-iG]-H=i[G,H]+O(\phi^2)\\=i\int d^d\pmb x\ \phi(\pmb x)[\rho(\pmb x),H]+O(\phi^2)\\=-\int d^d\pmb x\ \phi(\pmb x)\partial_t\rho(\pmb x)+O(\phi^2)$$

所以$$\partial_t\rho(\pmb x)+\pmb\nabla\cdot\pmb J(\pmb x)=0$$

## 问题4.3.4.
$$H=\frac1{2m}\int d^d\pmb x\ c^\dagger(\pmb x)(-i\partial_i+A_i(\pmb x))(-i\partial_i+A_i(\pmb x))c(\pmb x)\\+\gamma\int d^d\pmb x\ c^\dagger(\pmb x)(-i\partial_i+A_i(\pmb x))(-i\partial_i+A_i(\pmb x))\times\\(-i\partial_j+A_j(\pmb x))(-i\partial_j+A_j(\pmb x))c(\pmb x)$$

$$J^i(\pmb x)=\frac{\delta H}{\delta A_i(\pmb x)}=\frac1{2m}c^\dagger(\pmb x)(-i\partial_i+A_i(\pmb x))c(\pmb x)\\+\frac1{2m}(i\partial_i+A_i(\pmb x))c^\dagger(\pmb x)c(\pmb x)\\+\gamma c^\dagger(\pmb x)(-i\partial_i+A_i(\pmb x))(-i\partial_j+A_j(\pmb x))(-i\partial_j+A_j(\pmb x))c(\pmb x)\\+\gamma(i\partial_i+A_i(\pmb x))c^\dagger(\pmb x)(-i\partial_j+A_j(\pmb x))(-i\partial_j+A_j(\pmb x))c(\pmb x)\\+\gamma(i\partial_j+A_j(\pmb x))(i\partial_j+A_j(\pmb x))c^\dagger(\pmb x)(-i\partial_i+A_i(\pmb x))c(\pmb x)\\+\gamma(i\partial_j+A_j(\pmb x))(i\partial_j+A_j(\pmb x))(i\partial_i+A_i(\pmb x))c^\dagger(\pmb x)c(\pmb x)$$