# 《多体系统的量子场论》4.2.1草稿

(4.2.2)第三行忘了除以$Z$了
(4.2.6)有个$\dagger$的位置写错了

## 问题 4.2.1.
根据(4.2.6)
$$\mathcal G^\beta(\tau_1,\tau_2,\pmb k_1)\delta_{\pmb k_1,\pmb k_2}=\begin{cases}+\frac{{\rm Tr}(\exp[-\beta H]c_{\pmb k_1}(\tau_1)c_{\pmb k_2}^\dagger(\tau_2))}{{\rm Tr}(\exp[-\beta H])},{\rm for\ }\tau_1>\tau_2\\-\frac{{\rm Tr}(\exp[-\beta H]c_{\pmb k_2}^\dagger(\tau_2)c_{\pmb k_1}(\tau_1))}{{\rm Tr}(\exp[-\beta H])},{\rm for\ }\tau_1<\tau_2\end{cases}$$

考虑$-\beta<\tau<0$，于是
$$\mathcal G^\beta(\tau,\pmb k)=-\frac1Z{\rm Tr}[\exp[-\beta H]c_{\pmb k}^\dagger(0)c_{\pmb k}(\tau)]\\=-\frac1Z{\rm Tr}[\exp[-\beta H]c_{\pmb k}^\dagger\exp[\tau H]c_{\pmb k}\exp[-\tau H]]\\=-\frac1Z{\rm Tr}[\exp[\tau H]c_{\pmb k}\exp[-\tau H-\beta H]c_{\pmb k}^\dagger]$$

对于$\tau+\beta$，有：
$$\mathcal G^\beta(\tau+\beta,\pmb k)=\frac1Z{\rm Tr}[\exp[-\beta H]c_{\pmb k}(\tau+\beta)c_{\pmb k}^\dagger(0)]\\=\frac1Z{\rm Tr}[\exp[\tau H]c_{\pmb k}\exp[-\tau H-\beta H]c_{\pmb k}^\dagger]$$

根据(4.2.8)可知

$$\mathcal G^\beta(\omega_\gamma,\pmb k)=\int_0^\beta d\tau\ \mathcal G^\beta(\tau,\pmb k)\exp[i\omega_\gamma\tau]\\=(1-n_F(\xi_{\pmb k}))\int_0^\beta d\tau\ \exp[i\omega_\gamma\tau-\tau\xi_{\pmb k}]\\=(1-n_F(\xi_{\pmb k}))\frac{\exp[i\omega_\gamma\beta-\xi_{\pmb k}\beta]-1}{i\omega_\gamma-\xi_{\pmb k}}\\=\frac{-\exp[-\xi_{\pmb k}\beta]-1}{i\omega_\gamma-\xi_{\pmb k}}\frac{\exp[\beta\xi_{\pmb k}]}{\exp[\beta\xi_{\pmb k}]+1}\\=\frac{1}{-i\omega_\gamma+\xi_{\pmb k}}$$

## 问题 4.2.2.
根据(4.2.6)
$$\mathcal G^\beta(\tau_1,\tau_2,\pmb k_1)\delta_{\pmb k_1,\pmb k_2}=\begin{cases}+\frac{{\rm Tr}(\exp[-\beta H]c_{\pmb k_1}(\tau_1)c_{\pmb k_2}^\dagger(\tau_2))}{{\rm Tr}(\exp[-\beta H])},{\rm for\ }\tau_1>\tau_2\\-\frac{{\rm Tr}(\exp[-\beta H]c_{\pmb k_2}^\dagger(\tau_2)c_{\pmb k_1}(\tau_1))}{{\rm Tr}(\exp[-\beta H])},{\rm for\ }\tau_1<\tau_2\end{cases}$$

注意$[H,c_{\pmb k}]=-\xi_{\pmb k}c_{\pmb k},[H,c_{\pmb k}^\dagger]=\xi_{\pmb k}c_{\pmb k}^\dagger$

故
$$c_{\pmb k}(\tau)=\exp[\tau H]c_{\pmb k}\exp[-\tau H]=c_{\pmb k}\exp[-\xi_{\pmb k}\tau]$$

$$c_{\pmb k}^\dagger(\tau)=\exp[\tau H]c_{\pmb k}^\dagger\exp[-\tau H]=c_{\pmb k}^\dagger\exp[\xi_{\pmb k}\tau]$$

于是当$\beta>\tau>0$，有
$$\mathcal G^\beta(\tau,\pmb k)=\frac1Z{\rm Tr}[\exp[-\beta H]c_{\pmb k}(\tau)c_{\pmb k}^\dagger(0)]\\=\frac1Z{\rm Tr}[\exp[-\beta H]c_{\pmb k}c_{\pmb k}^\dagger]\exp[-\xi_{\pmb k}\tau]\\=\exp[-\xi_{\pmb k}\tau](1-\langle c_{\pmb k}^\dagger c_{\pmb k}\rangle)\\=\exp[-\xi_{\pmb k}\tau] (1-n_F(\xi_{\pmb k}))$$

当$0>\tau>-\beta$，有
$$\mathcal G^\beta(\tau,\pmb k)=-\frac1Z{\rm Tr}[\exp[-\beta H]c_{\pmb k}^\dagger(0)c_{\pmb k}(\tau)]\\=-\frac1Z{\rm Tr}[\exp[-\beta H]c_{\pmb k}^\dagger c_{\pmb k}]\exp[-\xi_{\pmb k}\tau]\\=-\exp[-\xi_{\pmb k}\tau]\langle c_{\pmb k}^\dagger c_{\pmb k}\rangle\\=-\exp[-\xi_{\pmb k}\tau]n_F(\xi_{\pmb k})$$

## 问题 4.2.3.
$$\beta^{-1}\int_0^\beta d\tau\ d\tau'\ \exp[i\omega_\gamma\tau-i\omega_\gamma'\tau']\mathcal G^\beta(\tau-\tau',\pmb k)\\=\beta^{-1}\int_0^\beta d\tau\ d\tau'\ \exp[i\omega_\gamma\tau-i\omega_\gamma'\tau']\\\times\beta^{-1}\sum_{\omega_\gamma''}\mathcal G^\beta(\omega_\gamma'',\pmb k)\exp[i\omega_\gamma''(\tau'-\tau)]\\=\sum_{\omega_\gamma''}\mathcal G^\beta(\omega_\gamma'',\pmb k)\delta_{\omega_\gamma,\omega_\gamma''}\delta_{\omega',\omega_\gamma''}\\=\mathcal G^\beta(\omega_\gamma,\pmb k)\delta_{\omega_\gamma,\omega_\gamma'}$$

## 问题 4.2.4.
$$c_{k_1}c_{k_2}^\dagger c_{k_3}c_{k_4}^\dagger=\delta_{k_1,k_2}c_{k_3}c_{k_4}^\dagger-c_{k_2}^\dagger c_{k_1}c_{k_3}c_{k_4}^\dagger\\=\delta_{k_1,k_2}\delta_{k_3,k_4}-\delta_{k_1,k_2}c_{k_4}^\dagger c_{k_3}-c_{k_2}^\dagger c_{k_1}\delta_{k_3,k_4}+c_{k_2}^\dagger c_{k_1}c_{k_4}^\dagger c_{k_3}\\=\delta_{k_1,k_2}\delta_{k_3,k_4}-\delta_{k_1,k_2}c_{k_4}^\dagger c_{k_3}-c_{k_2}^\dagger c_{k_1}\delta_{k_3,k_4}+\delta_{k_1,k_4}c_{k_2}^\dagger c_{k_3}\\-c_{k_2}^\dagger c_{k_4}^\dagger c_{k_1}c_{k_3}\\=\langle c_{k_1}c_{k_2}^\dagger\rangle\langle c_{k_3}c_{k_4}^\dagger\rangle+\langle c_{k_1}c_{k_2}^\dagger\rangle:c_{k_3}c_{k_4}^\dagger:+\langle c_{k_3}c_{k_4}^\dagger\rangle:c_{k_1}c_{k_2}^\dagger:\\+\langle c_{k_1}c_{k_4}^\dagger\rangle:c_{k_2}^\dagger c_{k_3}:+:c_{k_1}c_{k_2}^\dagger c_{k_3}c_{k_4}^\dagger:$$

$$c_{k_1}c_{k_2}c_{k_3}^\dagger c_{k_4}^\dagger=\delta_{k_2,k_3}c_{k_1}c_{k_4}^\dagger-c_{k_1}c_{k_3}^\dagger c_{k_2}c_{k_4}^\dagger\\=\delta_{k_2,k_3}\delta_{k_1,k_4}-\delta_{k_2,k_3}c_{k_4}^\dagger c_{k_1}-\delta_{k_1,k_3}c_{k_2}c_{k_4}^\dagger+c_{k_3}^\dagger c_{k_1}c_{k_2}c_{k_4}^\dagger\\=\delta_{k_2,k_3}\delta_{k_1,k_4}-\delta_{k_2,k_3}c_{k_4}^\dagger c_{k_1}-\delta_{k_1,k_3}\delta_{k_2,k_4}+\delta_{k_1,k_3}c_{k_4}^\dagger c_{k_2}\\+\delta_{k_2,k_4}c_{k_3}^\dagger c_{k_1}-c_{k_3}^\dagger c_{k_1}c_{k_4}^\dagger c_{k_2}\\=\delta_{k_2,k_3}\delta_{k_1,k_4}-\delta_{k_2,k_3}c_{k_4}^\dagger c_{k_1}-\delta_{k_1,k_3}\delta_{k_2,k_4}+\delta_{k_1,k_3}c_{k_4}^\dagger c_{k_2}\\+\delta_{k_2,k_4}c_{k_3}^\dagger c_{k_1}-\delta_{k_1,k_4}c_{k_3}^\dagger c_{k_2}+c_{k_3}^\dagger c_{k_4}^\dagger c_{k_1}c_{k_2}\\=\langle c_{k_1}c_{k_4}^\dagger\rangle\langle c_{k_2}c_{k_3}^\dagger\rangle+\langle c_{k_2}c_{k_3}^\dagger\rangle:c_{k_1}c_{k_4}^\dagger:-\langle c_{k_1}c_{k_3}^\dagger\rangle\langle c_{k_2}c_{k_4}^\dagger\rangle\\-\langle c_{k_1}c_{k_3}^\dagger\rangle:c_{k_2}c_{k_4}^\dagger:-\langle c_{k_2}c_{k_4}\rangle:c_{k_1}c_{k_3}^\dagger:+\langle c_{k_1}c_{k_4}^\dagger\rangle:c_{k_2}c_{k_3}^\dagger:\\+:c_{k_1}c_{k_2}c_{k_3}^\dagger c_{k_4}^\dagger:$$
