# 《多体系统的量子场论》2.1.1草稿

(2.1.2)的推导
$$G(x_b,x_a,t)=-i\langle x_b|\exp[-itp^2/2m]|x_a\rangle\\=-i\int dk\ \langle x_b|\exp[-itp^2/2m]|k\rangle\langle k|x_a\rangle\\=-i\int dk\ \exp[-itk^2/2m]\frac{1}{2\pi}\exp[ik(x_b-x_a)]\\=-\frac{i}{2\pi}\int dk\ \exp[-itk^2/2m+ik(x_b-x_a)]\\=-\frac{i}{2\pi}\sqrt{\frac{\pi}{it/2m}}\exp[im(x_b-x_a)^2/2t]\\=-i\sqrt{m/2\pi it}\exp[im(x_b-x_a)^2/2t]$$

## 问题2.1.1.
$$G(x_b,x_a,\omega)=\int_0^\infty dt\ G(x_b,x_a,t)\exp[it\omega-0^+t]\\=\int_0^\infty dt\ \sum_n\psi_n(x_b)\psi_n^*(x_a)(-i)\exp[it\omega-i\epsilon_nt-0^+t]\\=\sum_n\frac{\psi_n(x_b)\psi_n^*(x_a)}{\omega-\epsilon_n+i0^+}$$

对于谐振子：
考虑海森堡绘景下的算符方程：
$$\partial_tx_H(t)=-i[x_H(t),p_H^2(t)/2m]=p_H(t)/m\\\partial_tp_H(t)=-i[p_H(t),m\omega_0^2x_H^2(t)/2]=-m\omega_0^2x_H(t)$$

故
$$\begin{cases}x_H(t)=x\cos(\omega_0t)+\frac{p}{m\omega_0}\sin(\omega_0t)\\p_H(t)=p\cos(\omega_0t)-m\omega_0x\sin(\omega_0t)\end{cases}$$

于是
$$x_H(-t)=x\cos(\omega_0t)-\frac{p}{m\omega_0}\sin(\omega_0t)$$

于是
$$U(t)x=xU(t)\cos(\omega_0t)-\frac{pU(t)}{m\omega_0}\sin(\omega_0t)\\xU(t)=U(t)x\cos(\omega_0t)+\frac{U(t)p}{m\omega_0}\sin(\omega_0t)$$

于是
$$\frac{\sin(\omega_0t)}{m\omega_0}pU(t)=xU(t)\cos(\omega_0t)-U(t)x\\\frac{\sin(\omega_0t)}{m\omega_0}U(t)p=xU(t)-U(t)x\cos(\omega_0t)$$

于是
$$\frac{\sin(\omega_0t)}{m\omega_0}(-i)\partial_{x_b}\langle x_b|U(t)|x_a\rangle=(\cos(\omega_0t)x_b-x_a)\langle x_b|U(t)|x_a\rangle\\\frac{\sin(\omega_0t)}{m\omega_0}i\partial_{x_a}\langle x_b|U(t)|x_a\rangle=(x_b-\cos(\omega_0t)x_a)\langle x_b|U(t)|x_a\rangle$$

于是
$$\partial_{x_b}K=i\frac{m\omega_0}{\sin(\omega_0t)}(x_b\cos(\omega_0 t)-x_a)K\\\partial_{x_a}K=i\frac{m\omega_0}{\sin(\omega_0t)}(x_a\cos(\omega_0 t)-x_b)K$$

于是
$$\log K=i\frac{m\omega_0}{\sin(\omega_0t)}(x_b^2\cos(\omega_0 t)/2-x_ax_b)+f_1(x_a,t)\\\log K=i\frac{m\omega_0}{\sin(\omega_0t)}(x_a^2\cos(\omega_0 t)/2-x_ax_b)+f_2(x_b,t)$$

$$K=F_1(x_a,t)\exp\left[i\frac{m\omega_0}{\sin(\omega_0t)}(x_b^2\cos(\omega_0 t)/2-x_ax_b)\right]\\K=F_2(x_b,t)\exp\left[i\frac{m\omega_0}{\sin(\omega_0t)}(x_a^2\cos(\omega_0 t)/2-x_ax_b)\right]$$

取$x_a=x_b$可知$F_1=F_2$，故
$$F(x_a,t):\exp\left[i\frac{m\omega_0}{\sin(\omega_0t)}x_a^2\cos(\omega_0t)\right]\\=F(x_b,t):\exp\left[i\frac{m\omega_0}{\sin(\omega_0t)}x_b^2\cos(\omega_0t)\right]$$

从而$F(x,t)=\exp\left[i\frac{m\omega_0}{\sin(\omega_0t)}x^2\cos(\omega_0t)\right]R(t)$，所以

$$K=R(t)\exp\left[\frac{im\omega_0}{2\sin(\omega_0t)}((x_a^2+x_b^2)\cos(\omega_0t)-2x_ax_b)\right]$$

现在考虑求出$R(t)$，注意
$${\rm Tr\ }U(t)=\int dx\ K(x,x,t)\\=\int_{-\infty}^{+\infty}dx\ R(t)\exp\left[\frac{im\omega_0}{\sin(\omega_0t)}(x^2\cos(\omega_0t)-x^2)\right]\\=R(t)\int_{-\infty}^{+\infty}dx\ \exp[-im\omega_0\tan[\omega_0t/2]x^2]\\=R(t)\sqrt{\pi/im\omega_0\tan[\omega_0t/2]}$$

而
$${\rm Tr\ }U(t)=\sum_{n=0}^\infty\exp[-i(n+1/2)\omega_0t]\\=\exp[-i\omega_0t/2]\frac{1}{1-\exp[-i\omega_0t]}=\frac{1}{\exp[i\omega_0t/2]-\exp[-i\omega_0t/2]}\\=\frac{1}{2i\sin[\omega_0t/2]}$$

所以$R(t)=\sqrt{\frac{m\omega_0}{2i\pi\sin[\omega_0t]}}$

故$G(x_b,t,x_a,0)=(-i)\sqrt{\frac{m\omega_0}{2\pi i\sin[t\omega_0]}}\exp\left[\frac{im\omega_0}{2\sin(t\omega_0)}[(x_b^2+x_a^2)\cos(\omega_0t)-2x_ax_b]\right]$

现在考虑$G(0,t,0,0)=(-i)\sqrt{\frac{m\omega_0}{2\pi i\sin[t\omega_0]}}=-i\sqrt{\frac{m\omega_0}{\pi(\exp[it\omega_0]-\exp[-it\omega_0])}}\\=-i\sqrt{m\omega_0/\pi}\exp[-it\omega_0/2]\sqrt{1/(1-\exp[-2it\omega_0])}\\=-i\sqrt{m\omega_0/\pi}\exp[-it\omega_0/2](1-\exp[-2it\omega_0])^{-1/2}$

而
$$(1-x)^{-1/2}=\sum_{n=0}^\infty C_{-1/2}^{n}(-x)^n$$

故
$$G(0,t,0,0)\\=-i\sqrt{m\omega_0/\pi}\sum_{n=0}^\infty C_{-1/2}^n(-1)^n\exp[-(2n+1/2)it\omega_0]$$

从而
$$G(0,0,\omega)\\=-i\sqrt{m\omega_0/\pi}\sum_{n=0}^\infty C_{-1/2}^n(-1)^n\\\times\int_0^\infty dt\ \exp[-(2n+1/2)it\omega_0+it\omega-0^+t]\\=\sqrt{m\omega_0/\pi}\sum_{n=0}^\infty\frac{(-1)^nC_{-1/2}^n}{\omega-(2n+1/2)\omega_0+i0^+}$$

## 问题2.1.2.
$$G_E(\pmb k_b,\pmb k_a,\omega)\\=-i\int_0^\infty dt\ \exp[it\omega-0^+t]\langle\pmb k_b|\exp[-it\pmb p^2/2m]|\pmb k_a\rangle\\=-i\int_0^\infty dt\ \exp[it\omega-it\pmb k_a^2/2m-0^+t]\delta^{(3)}(\pmb k_b-\pmb k_a)\\=\frac{\delta^{(3)}(\pmb k_b-\pmb k_a)}{\omega-\pmb k_a^2/2m+i0^+}$$
